Lean4Lean/Verify/VLCtx.lean
@@ -36,12 +36,12 @@ def next : Option FVarId → Nat ⊕ FVarId → Option (Nat ⊕ FVarId)
   | none, .inr fv' => some (.inr fv')
   | some fv, .inr fv' => if fv == fv' then none else some (.inr fv')
 
-def find? : VLCtx → Nat ⊕ FVarId → Option (VLocalDecl × Nat)
+def find? : VLCtx → Nat ⊕ FVarId → Option (VExpr × VExpr)
   | [], _ => none
   | (ofv, d) :: Δ, v =>
     match next ofv v with
-    | none => some (d, 0)
-    | some v => do let (d', i) ← find? Δ v; some (d', i + d.depth)
+    | none => some (d.value, d.type)
+    | some v => do let (e, A) ← find? Δ v; some (e.liftN d.depth, A.liftN d.depth)
 
 def fvars (Δ : VLCtx) : List FVarId := Δ.filterMap (·.1)
 
@@ -49,5 +49,21 @@ def toCtx : VLCtx → List VExpr
   | [] => []
   | (_, .vlam ty) :: Δ => ty :: VLCtx.toCtx Δ
   | (_, .vlet _ _) :: Δ => VLCtx.toCtx Δ
+
+theorem lookup_isSome : ∀ {Δ : VLCtx}, (Δ.lookup (some fv)).isSome = (Δ.find? (.inr fv)).isSome
+  | [] => rfl
+  | (ofv, d) :: Δ => by
+    simp [List.lookup, find?, next]
+    cases ofv with
+    | none =>
+      simp [show (some fv == none) = false from rfl, lookup_isSome]
+      cases find? Δ (.inr fv) <;> simp [bind]
+    | some fv' =>
+      simp [show (some fv == some fv') = (fv == fv') from rfl, beq_comm fv]
+      cases fv' == fv <;> simp [lookup_isSome]
+      cases find? Δ (.inr fv) <;> simp [bind]
+
+theorem lookup_eq_none {Δ : VLCtx} : Δ.lookup (some fv) = none ↔ Δ.find? (.inr fv) = none := by
+  simp only [← Option.not_isSome_iff_eq_none, lookup_isSome]
 
 end VLCtx
